Teach WordProver something simple about less-than; split [allocated] definition into its own file; more TrivialArray, not yet with satisfactory automation

examples/Malloc.v
@@ -1,27 +1,11 @@
-Require Import AutoSep.
+Require Import AutoSep Allocated.
 Require Import Arith List.
+Export Allocated.
 
 Set Implicit Arguments.
 
 
 (** * Allocated memory regions with unknown contents *)
-
-Fixpoint allocated (base : W) (offset len : nat) : HProp :=
-  match len with
-    | O => Emp
-    | S len' => (Ex v, (match offset with
-                          | O => base
-                          | _ => base ^+ $(offset)
-                        end) =*> v) * allocated base (4+offset) len'
-  end%Sep.
-
-Notation "p =?> len" := (allocated p O len) (at level 39) : Sep_scope.
-
-Theorem allocated_extensional : forall base offset len, HProp_extensional (allocated base offset len).
-  destruct len; reflexivity.
-Qed.
-
-Local Hint Immediate allocated_extensional.
 
 Lemma allocated_shift_base' : forall base base' len offset offset',
   base ^+ $(offset) = base' ^+ $(offset')
