examples/TrivialArray.v
@@ -1,4 +1,4 @@
-Require Import AutoSep.
+Require Import AutoSep Allocated.
 
 (** * A trivial example to make sure the array proof automation isn't completely borked *)
 
@@ -6,15 +6,165 @@ Definition readS : assert := st ~> ExX, Ex ls, [| $3 < natToW (length ls) |]%wor
   /\ ![ ^[array ls st#Rv] * #0 ] st
   /\ st#Rp @@ (st' ~> [| st'#Rv = selN ls 3 |] /\ ![ ^[array ls st#Rv] * #1 ] st').
 
+Definition writeS : assert := st ~> ExX, Ex ls, [| $3 < natToW (length ls) |]%word
+  /\ ![ ^[array ls st#Rv] * #0 ] st
+  /\ st#Rp @@ (st' ~> ![ ^[array (updN ls 3 11) st#Rv] * #1 ] st').
+
+Definition bump := map (fun w : W => w ^+ $1).
+
+Definition bumpS : assert := st ~> ExX, Ex ls, Ex arr, Ex junk,
+  ![ (st#Sp ==*> arr, $(length ls), junk) * ^[array ls arr] * #0 ] st
+  /\ st#Rp @@ (st' ~> ![ ^[st#Sp =?> 3] * ^[array (bump ls) arr] * #1 ] st').
+
+Open Scope list_scope.
+
 Definition arrays := bmodule "read" {{
   bfunction "read" [readS] {
     Rv <- $[Rv + 12];;
     Goto Rp
+  } with bfunction "write" [writeS] {
+    $[Rv + 12] <- 11;;
+    Goto Rp
+  } with bfunction "bump" [bumpS] {
+    $[Sp+8] <- 0;;
+    [st ~> ExX, Ex ls, Ex done, Ex pending, Ex arr, Ex len, Ex i,
+      [| len = $(length ls) /\ i = $(length done) /\ ls = done ++ pending |]
+      /\ ![ (st#Sp ==*> arr, len, i) * ^[array ls arr] * #0 ] st
+      /\ st#Rp @@ (st' ~> Ex ls', [| ls' = done ++ bump pending |]
+        /\ ![ ^[st#Sp =?> 3] * ^[array ls' arr] * #1 ] st')]
+    While ($[Sp+8] < $[Sp+4]) {
+      Rv <- 4 * $[Sp+8];;
+      Rv <- $[Sp] + Rv;;
+      $[Rv] <- $[Rv] + 1;;
+      $[Sp+8] <- $[Sp+8] + 1
+    };;
+    Goto Rp
   }
 }}.
 
+Lemma length_nil : forall A, natToW 0 = $(length (@nil A)).
+  reflexivity.
+Qed.
+
+Lemma app_nil : forall A (ls : list A), ls = nil ++ ls.
+  reflexivity.
+Qed.
+
+Hint Immediate length_nil app_nil.
+
+Lemma shift_length : forall (done pending : list W),
+  ($(length done) : W) ^+ natToW 1
+  = $(length (done ++ (hd $0 pending ^+ natToW 1) :: nil)).
+  intros; rewrite app_length; simpl; subst.
+  autorewrite with sepFormula; reflexivity.
+Qed.
+
+Lemma shift_preserve : forall (done pending : list W),
+  ($(length done) : W) < $(length (done ++ pending))
+  -> done ++ pending = (done ++ hd $0 pending :: nil) ++ tl pending.
+  intros; subst; rewrite <- app_assoc; simpl.
+  destruct pending; simpl; try reflexivity.
+  rewrite app_nil_r in *; unfold natToW in *; nomega.
+Qed.
+
+Hint Resolve shift_preserve.
+
+Lemma shift_updN : forall v pending done,
+  (length pending > 0)%nat
+  -> updN (done ++ pending) (length done) v = (done ++ v :: nil) ++ tl pending.
+  induction done; simpl; intuition.
+  destruct pending; simpl in *; auto.
+  omega.
+Qed.
+
+Lemma shift_upd : forall v pending done,
+  natToW (length done) < $(length (done ++ pending))
+  -> (length (done ++ pending) < pow2 32)%nat
+  -> upd (done ++ pending) (length done) v = (done ++ v :: nil) ++ tl pending.
+  intros.
+  unfold upd.
+  rewrite wordToNat_natToWord_idempotent.
+  apply shift_updN; auto.
+  destruct pending; simpl.
+  rewrite <- app_nil_end in H.
+  clear H0.
+  unfold natToW in *.
+  nomega.
+  omega.
+
+  rewrite app_length in *.
+  assert (Datatypes.length done < pow2 32)%nat by omega.
+  apply Nlt_in.
+  rewrite Npow2_nat.
+  repeat rewrite Nat2N.id.
+  assumption.
+Qed.
+
+Theorem selN_hd : forall pending done,
+  selN (done ++ pending) (length done) = hd $0 pending.
+  induction done; simpl; intuition.
+  destruct pending; reflexivity.
+Qed.
+
+Theorem sel_hd : forall pending done,
+  (length (done ++ pending) < pow2 32)%nat
+  -> sel (done ++ pending) (length done) = hd $0 pending.
+  unfold sel; intros; subst.
+  rewrite wordToNat_natToWord_idempotent.
+  apply selN_hd.
+  rewrite app_length in *.
+  assert (Datatypes.length done < pow2 32)%nat by omega.
+  apply Nlt_in.
+  rewrite Npow2_nat.
+  repeat rewrite Nat2N.id.
+  assumption.
+Qed.
+
+Hint Resolve sel_hd.
+
+Lemma shift_reorg : forall done pending,
+  natToW (Datatypes.length done) < $ (Datatypes.length (done ++ pending))
+  -> (done ++ hd $0 pending ^+ $1 :: nil) ++ bump (tl pending)
+  = done ++ bump pending.
+  intros; rewrite DepList.pf_list_simpl.
+  destruct pending; simpl in *.
+  rewrite <- app_nil_end in *; unfold natToW in *; nomega.
+  reflexivity.
+Qed.
+
+Hint Resolve shift_reorg.
+
+Hint Extern 1 (_ = _) => apply shift_length || apply shift_upd.
+
+Lemma unbump : forall done pending,
+  ($ (length (done ++ pending)) : W) <= $ (length done)
+  -> (length (done ++ pending) < pow2 32)%nat
+  -> done ++ pending = done ++ bump pending.
+  intros; replace pending with (@nil W).
+  reflexivity.
+  destruct pending; auto; simpl length in *.
+  rewrite app_length in *.
+  simpl length in *.
+  pre_nomega.
+  repeat rewrite wordToN_nat in *.
+  repeat rewrite Nat2N.id in *.
+  rewrite wordToNat_natToWord_idempotent in *.
+  rewrite wordToNat_natToWord_idempotent in *.
+  elimtype False; omega.
+  apply Nlt_in.
+  rewrite Npow2_nat.
+  rewrite Nat2N.id.
+  assumption.
+  apply Nlt_in.
+  rewrite Npow2_nat.
+  rewrite Nat2N.id.
+  omega.
+Qed.
+
+Hint Resolve unbump.
+
 Theorem arraysOk : moduleOk arrays.
 (*TIME  Clear Timing Profile. *)
-  vcgen; abstract sep_auto.
+  vcgen; abstract (sep_auto; (subst; try rewrite sel_hd by eauto; eauto 7); sep_auto).
 (*TIME  Print Timing Profile. *)
 Qed.
