examples/Allocated.v
@@ -1,0 +1,19 @@
+Require Import AutoSep.
+
+
+Fixpoint allocated (base : W) (offset len : nat) : HProp :=
+  match len with
+    | O => Emp
+    | S len' => (Ex v, (match offset with
+                          | O => base
+                          | _ => base ^+ $(offset)
+                        end) =*> v) * allocated base (4+offset) len'
+  end%Sep.
+
+Notation "p =?> len" := (allocated p O len) (at level 39) : Sep_scope.
+
+Theorem allocated_extensional : forall base offset len, HProp_extensional (allocated base offset len).
+  destruct len; reflexivity.
+Qed.
+
+Hint Immediate allocated_extensional.
